proofs/Symcrust/Brute.lean
@@ -1,1 +1,1 @@
-import Symcrust.Brute.Brute2
+import Symcrust.Brute.Brute
