proofs/Symcrust/Brute/Brute.lean
@@ -2,6 +2,12 @@ import Lean
 import Aeneas
 import Symcrust.Brute.BruteLemmas
 
+/-  This file contains an experimental tactic which generalizes `brute` to allow arbitrary universal quantifiers
+    and more forms of upper bounds (rather than just `< b`, this `brute` is meant to support `≤ b` and even no upper
+    bound for finite types).
+
+    Note that this tactic is not yet functional, hence why it has not replaced the implementation defined in Brute.lean. -/
+
 open Lean Meta Parser Elab Tactic Aeneas Aeneas.Std
 
 initialize registerTraceClass `brute.debug
@@ -9,23 +15,46 @@ initialize registerTraceClass `brute.debug
 namespace Brute
 
 /-- A terminal tactic that attempts to prove goals of the form `∀ x y z ..., f x y z ...` via brute force.
-    This version of `brute` only supports goals consisting of a string of universally quantified upper-bounded
-    Nat-like types followed by a decidable function `f` (e.g. `∀ a < x₁, ∀ b < x₂ f a b` where the types of
-    `a` and `b` have `IsNatLike` instances). Additionally, this version of `brute` only supports goals with at most
-    five bounded quantifiers. -/
+    Brute requires that its goals consist of a string of universal quantifiers followed by a computable
+    function and that each of the universal quantifiers match one of the following forms:
+    - `∀ x : Nat, x < b → ...`
+    - `∀ x : Nat, x ≤ b → ...`
+    - `∀ x : BitVec n, ...`
+    - `∀ x : BitVec n, x < b → ...`
+    - `∀ x : BitVec n, x ≤ b → ...`
+    - `∀ x : UScalar _, ...`
+    - `∀ x : UScalar _, x < b → ...`
+    - `∀ x : UScalar _, x ≤ b → ...`
+
+    When a universal quantifier includes a `<` or `≤` condition, `brute` only checks over the values
+    below the given upper bound. When the universal quantifier does not include such a condition and
+    the type being quantified over is finite, `brute` checks over all values of the given type. -/
 syntax (name := brute) "brute" : tactic
 
-/-- A structure that holds info for binders of the form `∀ x < b, ...`-/
+inductive BoundType where
+  | ltUpperBound (b : Expr)
+  | leUpperBound (b : Expr)
+  | noUpperBound
+deriving Inhabited
+
+instance : ToMessageData BoundType where
+  toMessageData := fun
+    | .ltUpperBound b => m!"< {b}"
+    | .leUpperBound b => m!"≤ {b}"
+    | .noUpperBound => m!"no upper bound"
+
+/-- A structure that holds info for binders of the form `∀ x < b, ...` or `∀ x ≤ b, ...` or `∀ x, ...` -/
 structure BinderInfo where
-  x : FVarId -- The universally quantified variable.
-  b : Expr -- The value that the variable is upper bounded by. `b` cannot contain `x`
-  hxb : FVarId -- The variable whose type is `x < b`.
-  isNatLikeInst : Expr -- An Expr whose type is `IsNatLike t` where `x : t` and `b : t`.
+  x : FVarId -- The universally quantified variable
+  b : BoundType -- The value that the variable is upper bounded by
+  hxb : Option FVarId -- The variable whose type is `x < b` or `x ≤ b` (if present)
+  isNatLikeInst : Expr -- An Expr whose type is `IsNatLike t` where `x : t` and `b : t`
+deriving Inhabited
 
 instance : ToMessageData BinderInfo where
-  toMessageData := fun ⟨x, b, hxb, isNatLikeInst⟩ => m!"({Expr.fvar x}, {b}, {Expr.fvar hxb}, {isNatLikeInst})"
+  toMessageData := fun ⟨x, b, hxb, isNatLikeInst⟩ => m!"({Expr.fvar x}, {b}, {hxb.map Expr.fvar}, {isNatLikeInst})"
 
-/-- Retrieves the `UScalarTy` associated with a `U_` abbreviation -/
+/-- Retrieves the `UScalarTy` associated with a `U_` abbreviation. -/
 def getSizeTyFromAbbrev (t : Expr) : Option Expr :=
   match t with
   | .const ``U8 _ => some $ mkConst ``UScalarTy.U8
@@ -35,42 +64,34 @@ def getSizeTyFromAbbrev (t : Expr) : Option Expr :=
   | .const ``U128 _ => some $ mkConst ``UScalarTy.U128
   | _ => none
 
-/-- If `t` is an Expr corresponding to `Nat`, `BitVec n`, or `UScalar t'` (where `t' ≠ Usize`), then
-    `getIsNatLike` returns an Expr whose type is `IsNatLike t`. Otherwise, `getIsNatLike` returns `none`. -/
+def typeFromInst (inst : Expr) : TacticM Expr :=
+  match inst with
+  | .app (.app (.const ``IsNatLike.mk _) t) _ => pure t
+  | _ => throwError "{decl_name%} :: Invalid IsNatLike instance {inst}"
+
+/-- If `t` is an Expr corresponding to `Nat`, `BitVec n`, or `UScalar t'`, then `getIsNatLike` returns
+    an Expr whose type is `IsNatLike t`. Otherwise, `getIsNatLike` returns `none`. -/
 def getIsNatLikeInstance (t : Expr) : MetaM (Option Expr) := do
   match t with
   | .const ``Nat _ =>
-    -- `rflPf := (rfl : t = Nat)`
     let rflPf ← mkAppOptM ``Eq.refl #[some (.sort 1), some t]
-    -- `isNatPf := (isNatPf rflPf : IsNatLikePf t)`
     let isNatPf ← mkAppOptM ``IsNatLikePf.isNatPf #[none, rflPf]
-    -- `inst := (IsNatLike.mk isNatPf : IsNatLike t)`
     let inst ← mkAppM ``IsNatLike.mk #[isNatPf]
     return some inst
   | .app (.const ``BitVec _) n =>
-    -- `rflPf := (rfl : t = t)`
     let rflPf ← mkAppOptM ``Eq.refl #[some (.sort 1), some t]
-    -- `pSigmaβBody := (t = BitVec (Expr.bvar 0))`. This is not well typed until enclosed in a lambda
     let pSigmaβBody :=
       mkApp3 (mkConst ``Eq [2]) (.sort 1) (.app (.const ``BitVec []) n) (.app (.const ``BitVec []) (.bvar 0))
-    -- `pSigmaβ := (λ (n : Nat) => pSigmaβBody : ∀ n, Sort _)`
     let pSigmaβ := Expr.lam `n (mkConst ``Nat) pSigmaβBody .default
-    -- `pSigmaPf := (PSigma.mk n rflPf : PSigma pSigmaβ`
     let pSigmaPf ← mkAppOptM ``PSigma.mk #[none, some pSigmaβ, n, rflPf]
-    -- `isBitVecPf := (IsNatLikePf.isBitVecPf pSigmaPf : IsNatLikePf t)`
     let isBitVecPf ← mkAppOptM ``IsNatLikePf.isBitVecPf #[none, pSigmaPf]
-    -- `inst := (IsNatLike.mk isBitVecPf : IsNatLike t)`
     let inst ← mkAppM ``IsNatLike.mk #[isBitVecPf]
     return some inst
   | .app (.const ``UScalar _) (.const ``Usize _) => return none
   | .app (.const ``UScalar _) sizeTy => -- Matches with all `UScalar` types except `Usize`
-    -- `rflPf := (rfl : t = t)`
     let rflPf ← mkAppOptM ``Eq.refl #[some (.sort 1), some t]
-    -- `sizeTyNeUsizePf := (UScalarTy.noConfusion : sizeTy = Usize → False)`
     let sizeTyNeUsizePf ← mkAppOptM ``UScalarTy.noConfusion #[mkConst ``False, sizeTy, mkConst ``Usize]
-    -- `andPf : (⟨sizeTyNeUsizePf, rflPf⟩ : sizeTy = Usize → False ∧ t = t`
     let andPf ← mkAppM ``And.intro #[sizeTyNeUsizePf, rflPf]
-    -- `pSigmaβBody := (((Expr.bvar 0) ≠ Usize) ∧ (UScalar sizeTy = UScalar (Expr.bvar 0)))`. This is not well typed until enclosed in a lambda
     let pSigmaβBody :=
       mkApp2 (mkConst ``And)
         (mkApp3 (mkConst ``Ne [2]) (.sort 1) (.bvar 0) (mkConst ``Usize))
@@ -78,17 +99,12 @@ def getIsNatLikeInstance (t : Expr) : MetaM (Option Expr) := do
           (.app (.const ``UScalar []) sizeTy)
           (.app (.const ``UScalar []) (.bvar 0))
         )
-    -- `pSigmaβ := ((λ t' : UScalarTy => pSigmaβBody) : ∀ t', Sort _)`
-    let pSigmaβ := Expr.lam `t' (mkConst ``UScalarTy) pSigmaβBody .default
-    -- `pSigmaPf := (PSigma.mk sizeTy andPf : PSigma pSigmaβ)`
+    let pSigmaβ := Expr.lam `n (mkConst ``UScalarTy) pSigmaβBody .default
     let pSigmaPf ← mkAppOptM ``PSigma.mk #[none, pSigmaβ, sizeTy, andPf]
-    -- `isUScalarPf := (IsNatLikePf.isUScalarPf pSigmaPf : IsNatLikePf t)`
     let isUScalarPf ← mkAppOptM ``IsNatLikePf.isUScalarPf #[none, pSigmaPf]
-    -- `inst := (IsNatLike.mk isUScalarPf : IsNatLike t)`
     let inst ← mkAppM ``IsNatLike.mk #[isUScalarPf]
     return some inst
   | .const ``U8 _ | .const ``U16 _ | .const ``U32 _ | .const ``U64 _ | .const ``U128 _ =>
-    -- This code is identical to the preceding case except that `getSizeTyFromAbbrev` is called to obtain `sizeTy`
     let some sizeTy := getSizeTyFromAbbrev t
       | return none
     let rflPf ← mkAppOptM ``Eq.refl #[some (.sort 1), some t]
@@ -101,7 +117,7 @@ def getIsNatLikeInstance (t : Expr) : MetaM (Option Expr) := do
           (.app (.const ``UScalar []) sizeTy)
           (.app (.const ``UScalar []) (.bvar 0))
         )
-    let pSigmaβ := Expr.lam `t' (mkConst ``UScalarTy) pSigmaβBody .default
+    let pSigmaβ := Expr.lam `n (mkConst ``UScalarTy) pSigmaβBody .default
     let pSigmaPf ← mkAppOptM ``PSigma.mk #[none, pSigmaβ, sizeTy, andPf]
     let isUScalarPf ← mkAppOptM ``IsNatLikePf.isUScalarPf #[none, pSigmaPf]
     let inst ← mkAppM ``IsNatLike.mk #[isUScalarPf]
@@ -109,8 +125,9 @@ def getIsNatLikeInstance (t : Expr) : MetaM (Option Expr) := do
   | _ => return none
 
 /-- If `b1` has a NatLike type and `b2 : b1 < d` then returns a `BinderInfo` corresponding to
-    `b1`, `b1`'s Natlike type, and `b2`. Otherwise returns `none` -/
-def popBoundBinders (b1 b2 : FVarId) : TacticM (Option BinderInfo) := do
+    `b1`, `b1`'s Natlike type, and `b2`. Otherwise returns `none`. -/
+def popBoundBinders (poppedNatLikeGoalBinders : Array Expr)
+  (b1 b2 : FVarId) : TacticM (Option BinderInfo) := do
   let lctx ← getLCtx
   let some b1LocalDecl := lctx.find? b1
     | throwError "{decl_name%} :: Unable to find type of goal binder {Expr.fvar b1}"
@@ -120,171 +137,646 @@ def popBoundBinders (b1 b2 : FVarId) : TacticM (Option BinderInfo) := do
   let b2Type := b2LocalDecl.type
   let some isNatLikeInst ← getIsNatLikeInstance b1Type
     | return none -- Don't pop any binders if `b1`
-  let b1UpperBound ←
+  let (b1UpperBound, hxb) ←
     match b2Type with
     | .app (.app (.app (.app (.const ``LT.lt _) _) _) x) y =>
       if x != Expr.fvar b1 then return none
-      else pure y
-    | _ => return none
-  return some ⟨b1, b1UpperBound, b2, isNatLikeInst⟩
+      else
+        let abstractedY ← mkLambdaFVars poppedNatLikeGoalBinders y (binderInfoForMVars := .default)
+        pure (.ltUpperBound abstractedY, some b2)
+    | .app (.app (.app (.app (.const ``LE.le _) _) _) x) y =>
+      if x != Expr.fvar b1 then return none
+      else
+        let abstractedY ← mkLambdaFVars poppedNatLikeGoalBinders y (binderInfoForMVars := .default)
+        pure (.leUpperBound abstractedY, some b2)
+    | _ =>
+      if b1Type == mkConst ``Nat then return none -- Brute can't support unbounded Nats
+      else pure (.noUpperBound, none)
+  return some ⟨b1, b1UpperBound, hxb, isNatLikeInst⟩
 
-/-- Iterates through `goalBinders` and gathers as many pairs of binders of the form `∀ x < b` as `goalBinders`
-    allows. `popAllBoundBinders` then returns an array of the corresponding `BinderInfo`s. Note that the total
-    number of `goalBinders` may exceed the number of binder pairs gathered by `popBoundBinders` if `goalBinders`
-    contains binders that are not of the form `∀ x < b`.
-
-    For example, from the original goal `∀ x < b, ∀ y < x, ∀ z : Fin y, f x y z`, `goalBinders` would be
-    `#[x : Nat, hx : x < b, y : Nat, hy : y < x, z : Fin y]` and `popAllBoundBinders` would
-    return the BinderInfos for `(x, hx)` and `(y, hy)`. -/
-def popAllBoundBinders (goalBinders : Array FVarId) (acc : Array BinderInfo) : TacticM (Array BinderInfo) := do
-  match goalBinders with
+/-- Recursively calls `popBoundBinders` as many times as `goalBinders` allows. `poppedNatLikeGoalBinders`
+    contains all of the `goalBinders` popped so far which contain fvars with Natlike types (these
+    are exactly the fvars that need to be abstracted out of future upper bounds). -/
+def popAllBoundBinders (poppedNatLikeGoalBinders : Array Expr) (remainingGoalBinders : Array FVarId)
+  (acc : Array BinderInfo) : TacticM (Array BinderInfo) := do
+  match remainingGoalBinders with
+  | ⟨[b]⟩ =>
+    let lctx ← getLCtx
+    let some bLocalDecl := lctx.find? b
+      | throwError "{decl_name%} :: Unable to find type of goal binder {Expr.fvar b}"
+    let bType := bLocalDecl.type
+    let some isNatLikeInst ← getIsNatLikeInstance bType
+      | return acc -- Don't pop this last binder
+    let binderInfo := ⟨b, .noUpperBound, none, isNatLikeInst⟩
+    return acc.push binderInfo
   | ⟨b1 :: b2 :: restBinders⟩ =>
-    let some binderInfo ← popBoundBinders b1 b2
+    let some binderInfo ← popBoundBinders poppedNatLikeGoalBinders b1 b2
       | return acc
-    popAllBoundBinders ⟨restBinders⟩ $ acc.push binderInfo
+    if binderInfo.hxb.isSome then -- Two binders (`x` and `hxb` were popped)
+      popAllBoundBinders (poppedNatLikeGoalBinders.push (.fvar b1)) ⟨restBinders⟩ $ acc.push binderInfo
+    else -- Only one binder was popped
+      popAllBoundBinders (poppedNatLikeGoalBinders.push (.fvar b1)) ⟨b2 :: restBinders⟩ $ acc.push binderInfo
   | _ => return acc
+
+/-- Determines the optional upper bound that needs to be passed into `mkFold1` based on the BoundType `b` and
+    the relevant NatLikeInst `inst`. -/
+def upperBoundExprFromBoundType (b : BoundType) (inst : Expr) : TacticM Expr := do
+  match b with
+  | .ltUpperBound b => mkAppM ``some #[b]
+  | .leUpperBound b => mkAppOptM ``natLikeSucc #[none, inst, b]
+  | .noUpperBound => -- Return `none` of the appropriate type
+    match inst with
+    | .app (.app (.const ``IsNatLike.mk _) (.const ``Nat _)) _ =>
+      throwError "{decl_name%} :: Cannot derive an upper bound for type Nat"
+    | .app (.app (.const ``IsNatLike.mk _) t) _ =>
+      mkAppOptM ``none #[t]
+    | _ => throwError "{decl_name%} :: Invalid IsNatLike instance {inst}"
+
+/-- Applies the appropriate to derive the original goal from the successful computation of the fold function. -/
+def buildOfMkFoldProof (b : BoundType) (inst f f' hf : Expr) : TacticM Expr := do
+  match b with
+  | .ltUpperBound b => mkAppOptM ``ofMkFold1SomeLt #[none, inst, b, f, f', hf]
+  | .leUpperBound b => mkAppOptM ``ofMkFold1SomeLe #[none, inst, b, f, f', hf]
+  | .noUpperBound =>
+    match inst with
+    | .app (.app (.const ``IsNatLike.mk _) t) _ => mkAppOptM ``ofMkFold1None #[t, inst, f, f', hf]
+    | _ => throwError "{decl_name%} :: Invalid IsNatLike instance {inst}"
+
+def bruteBaseCase1 (xs : Array Expr) (g : Expr) (x : FVarId) (b : BoundType)
+  (hxbOpt : Option FVarId) (inst : Expr) : TacticM Expr := do
+  let boundFVars :=
+    match hxbOpt with
+    | some hxb => #[.fvar x, .fvar hxb]
+    | none => #[.fvar x]
+  let unboundFVars := xs.filter (fun fvar => !boundFVars.contains fvar)
+  let f ← mkLambdaFVars #[.fvar x] (← mkDecide (← mkForallFVars unboundFVars g)) (binderInfoForMVars := .default)
+  /- `hfPf` is one of the following (depending on the bound type of `b`):
+      - `(fun x hf => hf) : ∀ (x : t1), f x = true → f x = true`
+      - `(fun x hx hf => hf) : ∀ x < b, f x = true → f x = true`
+      - `(fun x hx hf => hf) : ∀ x ≤ b, f x = true → f x = true` -/
+  let hfPf ←
+    match b with
+    | .ltUpperBound b =>
+      match inst with
+      | .app (.app (.const ``IsNatLike.mk _) t) _ =>
+        let x ← mkFreshExprMVar t
+        let hxType ← mkAppM ``LT.lt #[x, b]
+        let hx ← mkFreshExprMVar hxType
+        let hfType ← mkAppM ``Eq #[← mkAppOptM' f #[x], mkConst ``true]
+        let hf ← mkFreshExprMVar hfType
+        mkLambdaFVars #[x, hx, hf] hf (binderInfoForMVars := .default)
+      | _ => throwError "{decl_name%} :: Invalid IsNatLike instance {inst}"
+    | .leUpperBound b =>
+      match inst with
+      | .app (.app (.const ``IsNatLike.mk _) t) _ =>
+        let x ← mkFreshExprMVar t
+        let hxType ← mkAppM ``LE.le #[x, b]
+        let hx ← mkFreshExprMVar hxType
+        let hfType ← mkAppM ``Eq #[← mkAppOptM' f #[x], mkConst ``true]
+        let hf ← mkFreshExprMVar hfType
+        mkLambdaFVars #[x, hx, hf] hf (binderInfoForMVars := .default)
+      | _ => throwError "{decl_name%} :: Invalid IsNatLike instance {inst}"
+    | .noUpperBound =>
+      match inst with
+      | .app (.app (.const ``IsNatLike.mk _) t) _ =>
+        let x ← mkFreshExprMVar t
+        let hfType ← mkAppM ``Eq #[← mkAppOptM' f #[x], mkConst ``true]
+        let hf ← mkFreshExprMVar hfType
+        mkLambdaFVars #[x, hf] hf (binderInfoForMVars := .default)
+      | _ => throwError "{decl_name%} :: Invalid IsNatLike instance {inst}"
+  let mkFold1Call ← mkAppOptM ``mkFold1 #[none, inst, ← upperBoundExprFromBoundType b inst, f, mkConst ``true]
+  let ofMkFoldProof ← buildOfMkFoldProof b inst f f hfPf
+
+  let levels := (collectLevelParams {} mkFold1Call).params.toList
+  let auxDeclName ← Term.mkAuxName `_brute
+  let decl := Declaration.defnDecl $
+    mkDefinitionValEx auxDeclName levels (mkConst ``Bool) mkFold1Call .abbrev .safe [auxDeclName]
+  addAndCompile decl
+
+  let rflPrf ← mkEqRefl (toExpr true)
+  let levelParams := levels.map .param
+  let foldResPf := mkApp3 (mkConst ``Lean.ofReduceBool) (mkConst auxDeclName levelParams) (toExpr true) rflPrf
+
+  let pf ← mkAppOptM' ofMkFoldProof $ Array.append #[foldResPf] (boundFVars.map some)
+  mkLambdaFVars boundFVars (binderInfoForMVars := .default) $ ← mkAppOptM ``of_decide_eq_true #[none, none, pf]
+
+-- **TODO** Modify names to make it clear that prefixBoundTypes, prefixInsts, and unusedPrefixMVars should have one-to-one correspondences with each other
+def buildComputationResBase_aux (prefixBoundTypes : List BoundType) (prefixInsts : Array Expr)
+  (usedPrefixMVars : Array Expr) (unusedPrefixMVars : Array Expr) (innerLamBody : Expr) : TacticM (Option Expr × Expr) := do
+  match prefixBoundTypes with
+  | [] => return (none, innerLamBody)
+  | nextPrefixBoundType :: prefixBoundTypes =>
+    let nextPrefixInst := prefixInsts[0]!
+    let prefixInsts := prefixInsts.drop 1
+    let nextPrefixMVar := unusedPrefixMVars[0]!
+    let unusedPrefixMVars := unusedPrefixMVars.drop 1
+
+    trace[brute.debug] "{decl_name%} :: nextPrefixMVar: {nextPrefixMVar}"
+    trace[brute.debug] "{decl_name%} :: nextPrefixMVar type: {← inferType nextPrefixMVar}"
+
+    match nextPrefixBoundType with
+    | .noUpperBound =>
+      let (_, innerLamBody) ← buildComputationResBase_aux prefixBoundTypes prefixInsts (usedPrefixMVars.push nextPrefixMVar) unusedPrefixMVars innerLamBody
+      let innerLam ← mkLambdaFVars #[nextPrefixMVar] innerLamBody (binderInfoForMVars := .default)
+      let res ← mkAppOptM ``mkFold1 #[none, nextPrefixInst, ← mkAppOptM ``none #[← inferType nextPrefixMVar], innerLam, mkConst ``true]
+      return (some innerLam, res)
+    | .ltUpperBound b =>
+      let (_, innerLamBody) ← buildComputationResBase_aux prefixBoundTypes prefixInsts (usedPrefixMVars.push nextPrefixMVar) unusedPrefixMVars innerLamBody
+      let innerLam ← mkLambdaFVars #[nextPrefixMVar] innerLamBody (binderInfoForMVars := .default)
+      let res ← mkAppOptM ``mkFold1 #[none, nextPrefixInst, ← mkAppM ``some #[← mkAppOptM' b (usedPrefixMVars.map some)], innerLam, mkConst ``true]
+      return (some innerLam, res)
+    | .leUpperBound b =>
+      let (_, innerLamBody) ← buildComputationResBase_aux prefixBoundTypes prefixInsts (usedPrefixMVars.push nextPrefixMVar) unusedPrefixMVars innerLamBody
+      let innerLam ← mkLambdaFVars #[nextPrefixMVar] innerLamBody (binderInfoForMVars := .default)
+      let res ← mkAppOptM ``mkFold1 #[none, nextPrefixInst, ← mkAppOptM ``natLikeSucc #[none, nextPrefixInst, ← mkAppOptM' b (usedPrefixMVars.map some)], innerLam, mkConst ``true]
+      return (some innerLam, res)
+
+def buildComputationResBase (prefixBinderInfos : Array BinderInfo)
+  (t f : Expr) (b : BoundType) (inst : Expr) : TacticM (Option Expr × Expr × Expr) := do
+  let prefixTypes ← prefixBinderInfos.mapM (fun bInfo => typeFromInst bInfo.isNatLikeInst)
+  let prefixBoundTypes := prefixBinderInfos.map (fun bInfo => bInfo.b)
+  let prefixInsts := prefixBinderInfos.map (fun bInfo => bInfo.isNatLikeInst)
+
+  let freshPrefixMVars ← prefixTypes.mapM (fun t => mkFreshExprMVar (some t))
+
+  trace[brute.debug] "{decl_name%} :: bp1"
+
+  -- `mkFold1 (some b1) (fun x' => mkFold1 (some (b2 x')) (f x') true) true = true`
+  -- `mkFold1 (some b1) (fun x' => mkFold1 none (f x') true) true = true`
+
+  /- Depending on b2, `innerLam` is either:
+      - `(fun (x' : t1) => mkFold1 (none : Option t2) (f x') true)`
+      - `(fun (x' : t1) => mkFold1 (some (b2 x')) (f x') true)` -/
+  let innerLamBody ← -- **TODO** Rename innerMostLam?
+    match b with
+    | .noUpperBound => mkAppOptM ``mkFold1 #[none, inst, ← mkAppOptM ``none #[t], ← mkAppOptM' f (freshPrefixMVars.map some), mkConst ``true]
+    | .ltUpperBound b => mkAppOptM ``mkFold1 #[none, inst, ← mkAppM ``some #[← mkAppOptM' b (freshPrefixMVars.map some)], ← mkAppOptM' f (freshPrefixMVars.map some), mkConst ``true]
+    | .leUpperBound b => mkAppOptM ``mkFold1 #[none, inst, ← mkAppOptM ``natLikeSucc #[none, inst, ← mkAppOptM' b (freshPrefixMVars.map some)], ← mkAppOptM' f (freshPrefixMVars.map some), mkConst ``true]
+
+  trace[brute.debug] "{decl_name%} :: bp2"
+  trace[brute.debug] "{decl_name%} :: innerLamBody: {innerLamBody}"
+  trace[brute.debug] "{decl_name%} :: innerLamBody type: {← inferType innerLamBody}"
+
+  /- Depending on b1, `mkFold1Call` is:
+    - `mkFold1 (none : Option t1) innerLam true`
+    - `mkFold1 (some b1) innerLam true` -/
+  let (fold1InnerLamOpt, mkFold1Call) ← buildComputationResBase_aux prefixBoundTypes.toList prefixInsts #[] freshPrefixMVars innerLamBody
+
+  trace[brute.debug] "{decl_name%} :: bp3"
+
+  let levels := (collectLevelParams {} mkFold1Call).params.toList
+  let auxDeclName ← Term.mkAuxName `_brute
+  let decl := Declaration.defnDecl $
+    mkDefinitionValEx auxDeclName levels (mkConst ``Bool) mkFold1Call .abbrev .safe [auxDeclName]
+  addAndCompile decl
+
+  trace[brute.debug] "{decl_name%} :: decl to be compiled: {mkFold1Call}"
+
+  let rflPrf ← mkEqRefl (toExpr true)
+  let levelParams := levels.map .param
+  return (fold1InnerLamOpt, mkFold1Call, mkApp3 (mkConst ``Lean.ofReduceBool) (mkConst auxDeclName levelParams) (toExpr true) rflPrf)
+
+def buildComputationResFinalRecursive (prefixFVars natLikeFVars : Array Expr) (prefixBinderInfos : Array BinderInfo)
+  (computationInnerLamOpt : Option Expr) (computationResIsTrue : Expr) : TacticM Expr := do
+  trace[brute.debug] "{decl_name%} :: bp1"
+  let computationInnerLam := computationInnerLamOpt.get!
+  let x' ← mkFreshExprMVar $ ← inferType natLikeFVars[0]!
+  let h ← mkFreshExprMVar $ ← mkAppM ``Eq #[← mkAppOptM' computationInnerLam #[x'], mkConst ``true]
+
+  match prefixBinderInfos[0]!.b with
+  | .noUpperBound =>
+    let arg3 ← mkLambdaFVars #[x', h] h (binderInfoForMVars := .default)
+    return ← mkAppOptM ``ofMkFold1None
+      #[none, prefixBinderInfos[0]!.isNatLikeInst, computationInnerLam, computationInnerLam, arg3, computationResIsTrue, natLikeFVars[0]!]
+  | .ltUpperBound b =>
+    let hx' ← mkFreshExprMVar $ ← mkAppM ``LT.lt #[x', b]
+    let arg3 ← mkLambdaFVars #[x', hx', h] h (binderInfoForMVars := .default)
+    return ← mkAppOptM ``ofMkFold1SomeLt
+      #[none, prefixBinderInfos[0]!.isNatLikeInst, b, computationInnerLam,
+        computationInnerLam, arg3, computationResIsTrue, natLikeFVars[0]!, prefixFVars[1]!]
+  | .leUpperBound b =>
+    let hx' ← mkFreshExprMVar $ ← mkAppM ``LE.le #[x', b]
+    let arg3 ← mkLambdaFVars #[x', hx', h] h (binderInfoForMVars := .default)
+    return ← mkAppOptM ``ofMkFold1SomeLe
+      #[none, prefixBinderInfos[0]!.isNatLikeInst, b, computationInnerLam,
+        computationInnerLam, arg3, computationResIsTrue, natLikeFVars[0]!, prefixFVars[1]!]
+
+def buildComputationResRecursive (allPrefixFVars natLikePrefixFVars : Array Expr)
+  (prefixBinderInfos suffixBinderInfos : Array BinderInfo)
+  (f : Expr) (computationInnerLamOpt : Option Expr)
+  (computationRes computationResIsTrue : Expr) : TacticM Expr := do -- **TODO** Generalize based on `b`
+  trace[brute.debug] "{decl_name%} :: natLikePrefixFVars at start: {natLikePrefixFVars}"
+  if hsize0 : natLikePrefixFVars.size <= 1 then
+    return computationResIsTrue
+  else
+    if hsize1 : natLikePrefixFVars.size == 2 then
+      return ← buildComputationResFinalRecursive allPrefixFVars natLikePrefixFVars prefixBinderInfos computationInnerLamOpt computationResIsTrue
+    else
+      let lastPrefixFVars :=
+        if prefixBinderInfos[prefixBinderInfos.size - 1]!.hxb.isSome then
+          #[allPrefixFVars[allPrefixFVars.size - 2]!, allPrefixFVars[allPrefixFVars.size - 1]!]
+        else
+          #[allPrefixFVars[allPrefixFVars.size - 1]!]
+      let secondLastPrefixFVars :=
+        if prefixBinderInfos[prefixBinderInfos.size - 2]!.hxb.isSome then
+          #[allPrefixFVars[allPrefixFVars.size - lastPrefixFVars.size - 2]!, allPrefixFVars[allPrefixFVars.size - lastPrefixFVars.size - 1]!]
+        else
+          #[allPrefixFVars[allPrefixFVars.size - lastPrefixFVars.size - 1]!]
+      let allPrefixFVarsTake1 := allPrefixFVars.take (allPrefixFVars.size - lastPrefixFVars.size)
+      let natLikePrefixFVarsTake1 := natLikePrefixFVars.take (natLikePrefixFVars.size - 1)
+      let natLikePrefixFVarsTake2 := natLikePrefixFVars.take (natLikePrefixFVars.size - 2)
+
+      let prefixTypes ← prefixBinderInfos.mapM (fun bInfo => typeFromInst bInfo.isNatLikeInst)
+      let prefixBoundTypes := prefixBinderInfos.map (fun bInfo => bInfo.b)
+      let prefixInsts := prefixBinderInfos.map (fun bInfo => bInfo.isNatLikeInst)
+
+      let suffixTypes ← suffixBinderInfos.mapM (fun bInfo => typeFromInst bInfo.isNatLikeInst)
+      let suffixBoundTypes := suffixBinderInfos.map (fun bInfo => bInfo.b)
+      let suffixInsts := suffixBinderInfos.map (fun bInfo => bInfo.isNatLikeInst)
+
+      let lastPrefixType := prefixTypes[prefixTypes.size - 1]!
+      let secondLastPrefixType := prefixTypes[prefixTypes.size - 2]!
+      let secondLastPrefixBoundType := prefixBoundTypes[prefixBoundTypes.size - 2]!
+      let lastPrefixInst := prefixInsts[prefixInsts.size - 1]!
+      let secondLastPrefixInst := prefixInsts[prefixInsts.size - 2]!
+      let lastPrefixBoundType := prefixBoundTypes[prefixBoundTypes.size - 1]!
+
+      let lastSuffixType := suffixTypes[suffixTypes.size - 1]!
+      let lastSuffixBoundType := suffixBoundTypes[suffixBoundTypes.size - 1]!
+      let lastSuffixInst := suffixInsts[suffixInsts.size - 1]!
+
+      let b := lastSuffixBoundType
+      let inst := lastSuffixInst
+      let t := lastSuffixType
+
+      let y' ← mkFreshExprMVar secondLastPrefixType
+      let z' ← mkFreshExprMVar lastPrefixType
+
+      trace[brute.debug] "{decl_name%} :: bp1"
+
+      trace[brute.debug] "{decl_name%} :: t: {t}"
+      trace[brute.debug] "{decl_name%} :: b: {b}"
+      trace[brute.debug] "{decl_name%} :: lastSuffixBoundType: {lastSuffixBoundType}"
+      trace[brute.debug] "{decl_name%} :: lastSuffixType: {lastSuffixType}"
+      trace[brute.debug] "{decl_name%} :: lastSuffixInst: {lastSuffixInst}"
+
+      let freshMVars := #[← mkFreshExprMVar secondLastPrefixType, ← mkFreshExprMVar lastPrefixType] ++
+        (← (suffixTypes.take (suffixTypes.size - 1)).mapM (fun t => mkFreshExprMVar (some t)))
+      let args := (natLikePrefixFVarsTake2 ++ freshMVars).map some
+      let innerLamBody ← -- **TODO** Rename innerMostLam?
+      match lastSuffixBoundType with
+      | .noUpperBound => mkAppOptM ``mkFold1 #[none, lastSuffixInst, ← mkAppOptM ``none #[lastSuffixType], ← mkAppOptM' f args, mkConst ``true]
+      | .ltUpperBound b => mkAppOptM ``mkFold1 #[none, lastSuffixInst, ← mkAppM ``some #[← mkAppOptM' b args], ← mkAppOptM' f args, mkConst ``true]
+      | .leUpperBound b => mkAppOptM ``mkFold1 #[none, lastSuffixInst, ← mkAppOptM ``natLikeSucc #[none, lastSuffixInst, ← mkAppOptM' b args], ← mkAppOptM' f args, mkConst ``true]
+      let (arg1Opt, _) ←
+        buildComputationResBase_aux ([secondLastPrefixBoundType, lastPrefixBoundType] ++ (suffixBoundTypes.take (suffixBoundTypes.size - 1)).toList)
+        (#[secondLastPrefixInst, lastPrefixInst] ++ (suffixInsts.take (suffixInsts.size - 1))) natLikePrefixFVarsTake2 freshMVars innerLamBody
+
+      let arg1 := arg1Opt.get!
+      let arg2 := arg1
+
+      trace[brute.debug] "{decl_name%} :: bp2"
+      trace[brute.debug] "{decl_name%} :: arg1: {arg1}"
+
+      -- `h : (fun y' => mkFold1 none (fun z' => mkFold1 none (f x y' z') true) true) y' = true`
+      let h ← mkFreshExprMVar $ ← mkAppM ``Eq #[← mkAppOptM' arg1 #[y'], mkConst ``true]
+
+      trace[brute.debug] "{decl_name%} :: bp2.5"
+      trace[brute.debug] "y': {y'}"
+      trace[brute.debug] "{decl_name%} :: natLikePrefixFVars: {natLikePrefixFVars}"
+
+      -- `arg3 = (fun _ h => h)` or `arg3 = (fun y' hy' h => h)`
+      let arg3 ←
+        match prefixBinderInfos[prefixBinderInfos.size - 2]!.b with
+        | .noUpperBound => mkLambdaFVars #[y', h] h (binderInfoForMVars := .default)
+        | .ltUpperBound b =>
+          let hy' ← mkFreshExprMVar $ ← mkAppM ``LT.lt #[y', ← mkAppOptM' b ((natLikePrefixFVars.take (natLikePrefixFVars.size - 2)).map some)]
+          mkLambdaFVars #[y', hy', h] h (binderInfoForMVars := .default)
+        | .leUpperBound b =>
+          let hy' ← mkFreshExprMVar $ ← mkAppM ``LE.le #[y', ← mkAppOptM' b ((natLikePrefixFVars.take (natLikePrefixFVars.size - 2)).map some)]
+          mkLambdaFVars #[y', hy', h] h (binderInfoForMVars := .default)
+
+      trace[brute.debug] "{decl_name%} :: bp3"
+
+      let arg4 ←
+        buildComputationResRecursive allPrefixFVarsTake1 natLikePrefixFVarsTake1 (prefixBinderInfos.take (prefixBinderInfos.size - 1))
+          (prefixBinderInfos[prefixBinderInfos.size - 1]! :: suffixBinderInfos.toList).toArray
+          f computationInnerLamOpt computationRes computationResIsTrue
+
+      trace[brute.debug] "{decl_name%} :: bp4"
+
+      match secondLastPrefixBoundType with
+      | .noUpperBound => mkAppOptM ``ofMkFold1None $ #[none, secondLastPrefixInst, arg1, arg2, arg3, arg4] ++ (secondLastPrefixFVars.map some)
+      | .ltUpperBound b =>
+        mkAppOptM ``ofMkFold1SomeLt $
+          #[none, secondLastPrefixInst, ← mkAppOptM' b ((natLikePrefixFVars.take (natLikePrefixFVars.size - 2)).map some), arg1, arg2, arg3, arg4] ++ (secondLastPrefixFVars.map some)
+      | .leUpperBound b =>
+        mkAppOptM ``ofMkFold1SomeLe $
+          #[none, secondLastPrefixInst, ← mkAppOptM' b ((natLikePrefixFVars.take (natLikePrefixFVars.size - 2)).map some), arg1, arg2, arg3, arg4] ++ (secondLastPrefixFVars.map some)
+termination_by natLikePrefixFVars.size
+decreasing_by
+  simp only [not_le, beq_iff_eq] at hsize0 hsize1
+  simp
+  omega
+
+def buildArg3 (prefixFVars natLikeFVars : Array Expr) (prefixBinderInfos : Array BinderInfo) (finalBinderInfo : BinderInfo)
+  (f : Expr) (computationInnerLamOpt : Option Expr)
+  (computationRes computationResIsTrue : Expr) : TacticM Expr := do
+  let b := finalBinderInfo.b
+  let inst := finalBinderInfo.isNatLikeInst
+  let t ← typeFromInst inst
+
+  let lastPrefixFVars :=
+    if prefixBinderInfos[prefixBinderInfos.size - 1]!.hxb.isSome then
+      #[prefixFVars[prefixFVars.size - 2]!, prefixFVars[prefixFVars.size - 1]!]
+    else
+      #[prefixFVars[prefixFVars.size - 1]!]
+  let natLikeFVarsTaken := natLikeFVars.take (natLikeFVars.size - 1)
+
+  let prefixTypes ← prefixBinderInfos.mapM (fun bInfo => typeFromInst bInfo.isNatLikeInst)
+  let prefixBoundTypes := prefixBinderInfos.map (fun bInfo => bInfo.b)
+  let prefixInsts := prefixBinderInfos.map (fun bInfo => bInfo.isNatLikeInst)
+
+  let lastPrefixType := prefixTypes[prefixTypes.size - 1]!
+  let lastPrefixBoundType := prefixBoundTypes[prefixBoundTypes.size - 1]!
+  let lastPrefixInst := prefixInsts[prefixInsts.size - 1]!
+
+  let x' ← mkFreshExprMVar lastPrefixType
+
+  match b with
+  | .noUpperBound =>
+    trace[brute.debug] "{decl_name%} :: bp1"
+
+    -- `arg1 = (fun (x' : t1) => mkFold1 (none : Option t2) (fun (_ : t2) => mkFold1 none (f x') true) true)`
+    let arg1InnerLamBody ← mkAppOptM ``mkFold1 #[none, inst, ← mkAppOptM ``none #[t], ← mkAppOptM' f ((natLikeFVarsTaken.push x').map some), mkConst ``true]
+    let arg1InnerLam ← mkLambdaFVars #[← mkFreshExprMVar t] arg1InnerLamBody (binderInfoForMVars := .default)
+    let arg1LamBody ← mkAppOptM ``mkFold1 #[none, inst, ← mkAppOptM ``none #[t], arg1InnerLam, mkConst ``true]
+    let arg1 ← mkLambdaFVars #[x'] arg1LamBody (binderInfoForMVars := .default)
+
+    trace[brute.debug] "{decl_name%} :: bp2"
+
+    -- `arg2 = (fun (x' : t1) => mkFold1 none (f x') true)`
+    let arg2LamBody ← mkAppOptM ``mkFold1 #[none, inst, ← mkAppOptM ``none #[t], ← mkAppOptM' f ((natLikeFVarsTaken.push x').map some), mkConst ``true]
+    let arg2 ← mkLambdaFVars #[x'] arg2LamBody (binderInfoForMVars := .default)
+
+    trace[brute.debug] "{decl_name%} :: bp3"
+
+    /- Depending on `lastPrefixBoundType`, `arg3` is equal to:
+      - `(fun (x' : t1) => ofMkFold1Triv f x' (none : Option t2))`
+      - `(fun (x' : t1) (hx' : x' < b1) => ofMkFold1Triv f x' (none : Option t2))`
+      - `(fun (x' : t1) (hx' : x' ≤ b1) => ofMkFold1Triv f x' (none : Option t2))` -/
+    let arg3LamBody ← mkAppOptM ``ofMkFold1Triv #[none, none, lastPrefixInst, inst, ← mkAppOptM' f ((natLikeFVarsTaken.push x').map some), x', ← mkAppOptM ``none #[t]]
+    let arg3 ←
+      match lastPrefixBoundType with
+      | .noUpperBound => mkLambdaFVars #[x'] arg3LamBody (binderInfoForMVars := .default)
+      | .ltUpperBound b1 =>
+        let hx' ← mkFreshExprMVar $ ← mkAppOptM ``LT.lt #[lastPrefixType, none, x', ← mkAppOptM' b1 ((natLikeFVarsTaken.push x').map some)]
+        mkLambdaFVars #[x', hx'] arg3LamBody (binderInfoForMVars := .default)
+      | .leUpperBound b1 =>
+        let hx' ← mkFreshExprMVar $ ← mkAppOptM ``LE.le #[lastPrefixType, none, x', ← mkAppOptM' b1 ((natLikeFVarsTaken.push x').map some)]
+        mkLambdaFVars #[x', hx'] arg3LamBody (binderInfoForMVars := .default)
+
+    trace[brute.debug] "{decl_name%} :: bp4"
+
+    let computationResIsTrue ←
+      buildComputationResRecursive prefixFVars natLikeFVars prefixBinderInfos #[finalBinderInfo] f computationInnerLamOpt computationRes computationResIsTrue
+
+    match lastPrefixBoundType with
+    | .noUpperBound =>
+      let ofMkFold1Res ← mkAppOptM ``ofMkFold1None #[lastPrefixType, lastPrefixInst, arg1, arg2, arg3, computationResIsTrue]
+      mkAppM' ofMkFold1Res lastPrefixFVars
+    | .ltUpperBound b1 =>
+      let ofMkFold1Res ← mkAppOptM ``ofMkFold1SomeLt #[lastPrefixType, lastPrefixInst, ← mkAppOptM' b1 (natLikeFVarsTaken.map some), arg1, arg2, arg3, computationResIsTrue]
+      mkAppM' ofMkFold1Res lastPrefixFVars
+    | .leUpperBound b1 =>
+      let ofMkFold1Res ← mkAppOptM ``ofMkFold1SomeLe #[lastPrefixType, lastPrefixInst, ← mkAppOptM' b1 (natLikeFVarsTaken.map some), arg1, arg2, arg3, computationResIsTrue]
+      mkAppM' ofMkFold1Res lastPrefixFVars
+  | .ltUpperBound b =>
+    trace[brute.debug] "{decl_name%} :: bp1"
+
+    -- `arg1 = (fun (x' : t1) => mkFold1 (some (b x')) (fun (_ : t2) => mkFold1 (some (b x')) (f x') true) true)`
+    let arg1InnerLamBody ← mkAppOptM ``mkFold1 #[none, inst, ← mkAppM ``some #[← mkAppOptM' b ((natLikeFVarsTaken.push x').map some)], ← mkAppOptM' f ((natLikeFVarsTaken.push x').map some), mkConst ``true]
+    let arg1InnerLam ← mkLambdaFVars #[← mkFreshExprMVar t] arg1InnerLamBody (binderInfoForMVars := .default)
+    let arg1LamBody ← mkAppOptM ``mkFold1 #[none, inst, ← mkAppM ``some #[← mkAppOptM' b ((natLikeFVarsTaken.push x').map some)], arg1InnerLam, mkConst ``true]
+    let arg1 ← mkLambdaFVars #[x'] arg1LamBody (binderInfoForMVars := .default)
+
+    trace[brute.debug] "{decl_name%} :: bp2"
+
+    -- `arg2 = (fun (x' : t1) => mkFold1 (some (b2 x')) (f x') true)`
+    let arg2LamBody ← mkAppOptM ``mkFold1 #[none, inst, ← mkAppM ``some #[← mkAppOptM' b ((natLikeFVarsTaken.push x').map some)], ← mkAppOptM' f ((natLikeFVarsTaken.push x').map some), mkConst ``true]
+    let arg2 ← mkLambdaFVars #[x'] arg2LamBody (binderInfoForMVars := .default)
+
+    trace[brute.debug] "{decl_name%} :: bp3"
+
+    /- Depending on `b1`, `arg3` is equal to:
+      - `(fun (x' : t1) => ofMkFold1Triv f x' (some (b2 x')))`
+      - `(fun (x' : t1) (hx' : x' < b1) => ofMkFold1Triv f x' (some (b2 x')))`
+      - `(fun (x' : t1) (hx' : x' ≤ b1) => ofMkFold1Triv f x' (some (b2 x')))` -/
+    let arg3LamBody ←
+      mkAppOptM ``ofMkFold1Triv #[none, none, lastPrefixInst, inst, ← mkAppOptM' f (natLikeFVarsTaken.map some), x', ← mkAppM ``some #[← mkAppOptM' b ((natLikeFVarsTaken.push x').map some)]]
+    let arg3 ←
+      match lastPrefixBoundType with
+      | .noUpperBound => mkLambdaFVars #[x'] arg3LamBody (binderInfoForMVars := .default)
+      | .ltUpperBound b1 =>
+        let hx' ← mkFreshExprMVar $ ← mkAppOptM ``LT.lt #[lastPrefixType, none, x', ← mkAppOptM' b1 (natLikeFVarsTaken.map some)]
+        mkLambdaFVars #[x', hx'] arg3LamBody (binderInfoForMVars := .default)
+      | .leUpperBound b1 =>
+        let hx' ← mkFreshExprMVar $ ← mkAppOptM ``LE.le #[lastPrefixType, none, x', ← mkAppOptM' b1 (natLikeFVarsTaken.map some)]
+        mkLambdaFVars #[x', hx'] arg3LamBody (binderInfoForMVars := .default)
+
+    trace[brute.debug] "{decl_name%} :: bp4"
+
+    let computationResIsTrue ←
+      buildComputationResRecursive prefixFVars natLikeFVars prefixBinderInfos #[finalBinderInfo] f computationInnerLamOpt computationRes computationResIsTrue
+
+    match lastPrefixBoundType with
+    | .noUpperBound =>
+      let ofMkFold1Res ← mkAppOptM ``ofMkFold1None #[lastPrefixType, lastPrefixInst, arg1, arg2, arg3, computationResIsTrue]
+      mkAppM' ofMkFold1Res lastPrefixFVars
+    | .ltUpperBound b1 =>
+      let ofMkFold1Res ← mkAppOptM ``ofMkFold1SomeLt #[lastPrefixType, lastPrefixInst, ← mkAppOptM' b1 (natLikeFVarsTaken.map some), arg1, arg2, arg3, computationResIsTrue]
+      mkAppM' ofMkFold1Res lastPrefixFVars
+    | .leUpperBound b1 =>
+      let ofMkFold1Res ← mkAppOptM ``ofMkFold1SomeLe #[lastPrefixType, lastPrefixInst, ← mkAppOptM' b1 (natLikeFVarsTaken.map some), arg1, arg2, arg3, computationResIsTrue]
+      mkAppM' ofMkFold1Res lastPrefixFVars
+  | .leUpperBound b =>
+    -- `arg1 = (fun (x' : t1) => mkFold1 (natLikeSucc (b2 x')) (fun (_ : t2) => mkFold1 (natLikeSucc (b2 x')) (f x') true) true)`
+    let arg1InnerLamBody ←
+      mkAppOptM ``mkFold1 #[none, inst, ← mkAppOptM ``natLikeSucc #[none, inst, ← mkAppOptM' b ((natLikeFVarsTaken.push x').map some)], ← mkAppOptM' f ((natLikeFVarsTaken.push x').map some), mkConst ``true]
+    let arg1InnerLam ← mkLambdaFVars #[← mkFreshExprMVar t] arg1InnerLamBody (binderInfoForMVars := .default)
+    let arg1LamBody ←
+      mkAppOptM ``mkFold1 #[none, inst, ← mkAppOptM ``natLikeSucc #[none, inst, ← mkAppOptM' b ((natLikeFVarsTaken.push x').map some)], arg1InnerLam, mkConst ``true]
+    let arg1 ← mkLambdaFVars #[x'] arg1LamBody (binderInfoForMVars := .default)
+
+    -- `arg2 = (fun (x' : t1) => mkFold1 (natLikeSucc (b2 x')) (f x') true)`
+    let arg2LamBody ←
+      mkAppOptM ``mkFold1 #[none, inst, ← mkAppOptM ``natLikeSucc #[none, inst, ← mkAppOptM' b ((natLikeFVarsTaken.push x').map some)], ← mkAppOptM' f ((natLikeFVarsTaken.push x').map some), mkConst ``true]
+    let arg2 ← mkLambdaFVars #[x'] arg2LamBody (binderInfoForMVars := .default)
+
+    /- Depending on `b1`, `arg3` is equal to:
+      - `(fun (x' : t1) => ofMkFold1Triv f x' (natLikeSucc (b2 x')))`
+      - `(fun (x' : t1) (hx' : x' < b1) => ofMkFold1Triv f x' (natLikeSucc (b2 x')))`
+      - `(fun (x' : t1) (hx' : x' ≤ b1) => ofMkFold1Triv f x' (natLikeSucc (b2 x')))` -/
+    let arg3LamBody ←
+      mkAppOptM ``ofMkFold1Triv
+        #[none, none, lastPrefixInst, inst, ← mkAppOptM' f (natLikeFVarsTaken.map some), x', ← mkAppOptM ``natLikeSucc #[none, inst, ← mkAppOptM' b ((natLikeFVarsTaken.push x').map some)]]
+    let arg3 ←
+      match lastPrefixBoundType with
+      | .noUpperBound => mkLambdaFVars #[x'] arg3LamBody (binderInfoForMVars := .default)
+      | .ltUpperBound b1 =>
+        let hx' ← mkFreshExprMVar $ ← mkAppOptM ``LT.lt #[lastPrefixType, none, x', ← mkAppOptM' b1 (natLikeFVarsTaken.map some)]
+        mkLambdaFVars #[x', hx'] arg3LamBody (binderInfoForMVars := .default)
+      | .leUpperBound b1 =>
+        let hx' ← mkFreshExprMVar $ ← mkAppOptM ``LE.le #[lastPrefixType, none, x', ← mkAppOptM' b1 (natLikeFVarsTaken.map some)]
+        mkLambdaFVars #[x', hx'] arg3LamBody (binderInfoForMVars := .default)
+
+    let computationResIsTrue ←
+      buildComputationResRecursive prefixFVars natLikeFVars prefixBinderInfos #[finalBinderInfo] f
+        computationInnerLamOpt computationRes computationResIsTrue
+
+    match lastPrefixBoundType with
+    | .noUpperBound =>
+      let ofMkFold1Res ← mkAppOptM ``ofMkFold1None #[lastPrefixType, lastPrefixInst, arg1, arg2, arg3, computationResIsTrue]
+      mkAppM' ofMkFold1Res lastPrefixFVars
+    | .ltUpperBound b1 =>
+      let ofMkFold1Res ← mkAppOptM ``ofMkFold1SomeLt #[lastPrefixType, lastPrefixInst, ← mkAppOptM' b1 (natLikeFVarsTaken.map some), arg1, arg2, arg3, computationResIsTrue]
+      mkAppM' ofMkFold1Res lastPrefixFVars
+    | .leUpperBound b1 =>
+      let ofMkFold1Res ← mkAppOptM ``ofMkFold1SomeLe #[lastPrefixType, lastPrefixInst, ← mkAppOptM' b1 (natLikeFVarsTaken.map some), arg1, arg2, arg3, computationResIsTrue]
+      mkAppM' ofMkFold1Res lastPrefixFVars
+
+def bruteCore (binderInfos : Array BinderInfo) (unboundBinders : Array Expr) (g : Expr) : TacticM Expr := do
+  let finalBinderInfo := binderInfos[binderInfos.size - 1]!
+  let finalBinderFVars :=
+    match finalBinderInfo.hxb with
+    | some hxb => #[Expr.fvar finalBinderInfo.x, Expr.fvar hxb]
+    | none => #[Expr.fvar finalBinderInfo.x]
+  let t ← typeFromInst finalBinderInfo.isNatLikeInst
+  let inst := finalBinderInfo.isNatLikeInst
+
+  trace[brute.debug] "bp1"
+
+  let binderInfosPrefix := binderInfos.take (binderInfos.size - 1)
+  let natLikeFVars := binderInfos.map (fun bInfo => Expr.fvar bInfo.x)
+  let prefixNatLikeFVars := binderInfosPrefix.map (fun bInfo => Expr.fvar bInfo.x)
+  let prefixFVars := Array.flatten $
+    binderInfosPrefix.map
+    (fun bInfo =>
+      match bInfo.hxb with
+      | some hxb => #[Expr.fvar bInfo.x, Expr.fvar hxb]
+      | none => #[Expr.fvar bInfo.x])
+
+  trace[brute.debug] "bp2"
+
+  let f ← mkLambdaFVars natLikeFVars (← mkDecide (← mkForallFVars unboundBinders g)) (binderInfoForMVars := .default)
+  let fWithPrefix ← mkAppOptM' f (prefixNatLikeFVars.map some)
+
+  trace[brute.debug] "bp3"
+
+  /- `arg1` is one of the following (depending on the bound type of finalBinderInfo)
+      - `(fun (_ : t) => mkFold1 (none : Option t) fWithPrefix true) : t → Bool`
+      - `(fun (_ : t) => mkFold1 (some (finalBinderInfo.b prefixNatLikeFVars)) fWithPrefix true)`
+      - `(fun (_ : t) => mkFold1 (natLikeSucc (finalBinderInfo.b prefixNatLikeFVars)) fWithPrefix true)` -/
+  let arg1 ←
+    match finalBinderInfo.b with
+    | .noUpperBound =>
+      let lamBody ←
+        mkAppOptM ``mkFold1
+          #[none, inst, ← mkAppOptM ``none #[t], fWithPrefix, mkConst ``true]
+      pure $ Expr.lam `_ t lamBody .default
+    | .ltUpperBound b =>
+      let lamBody ←
+        mkAppOptM ``mkFold1
+          #[none, inst, ← mkAppM ``some #[← mkAppOptM' b (prefixNatLikeFVars.map some)], fWithPrefix, mkConst ``true]
+      pure $ Expr.lam `_ t lamBody .default
+    | .leUpperBound b =>
+      let lamBody ←
+        mkAppOptM ``mkFold1
+          #[none, inst, ← mkAppOptM ``natLikeSucc #[none, inst, ← mkAppOptM' b (prefixNatLikeFVars.map some)], fWithPrefix, mkConst ``true]
+      pure $ Expr.lam `_ t lamBody .default
+
+  trace[brute.debug] "bp4"
+
+  /- `arg2` is one of the following (depending on the bound type of finalBinderInfo)
+      - `(fun (y : t) (h : arg1 y = true) => ofMkFold1None (f x) (f x) (fun (y' : t) (hf : f x y' = true) => hf) h y)`
+      - `(fun (y : t) (hy : y < (b2 x)) (h : arg1 y = true) =>`
+            `ofMkFold1SomeLt (b2 x) (f x) (f x) (fun (y' : t) (hy' : y' < b2 x) (hf : f x y' = true) => hf) h y hy)`
+      - `(fun (y : t) (hy : y ≤ (b2 x)) (h : arg1 y = true) =>`
+            `ofMkFold1SomeLe (b2 x) (f x) (f x) (fun (y' : t) (hy' : y' ≤ b2 x) (hf : f x y' = true) => hf) h y hy)` -/
+  let arg2 ←
+    match finalBinderInfo.b with
+    | .noUpperBound =>
+      let y ← mkFreshExprMVar t
+      let y' ← mkFreshExprMVar t
+      let h ← mkFreshExprMVar $ ← mkAppM ``Eq #[← mkAppOptM' arg1 #[y], mkConst ``true]
+      let hf ← mkFreshExprMVar $ ← mkAppM ``Eq #[← mkAppOptM' fWithPrefix #[y'], mkConst ``true]
+      let innerLam ← mkLambdaFVars #[y', hf] hf (binderInfoForMVars := .default)
+      let lamBody ← mkAppOptM ``ofMkFold1None #[none, inst, fWithPrefix, fWithPrefix, innerLam, h, y]
+      mkLambdaFVars #[y, h] lamBody (binderInfoForMVars := .default)
+    | .ltUpperBound b =>
+      let y ← mkFreshExprMVar t
+      let y' ← mkFreshExprMVar t
+      let hy ← mkFreshExprMVar $ ← mkAppM ``LT.lt #[y, ← mkAppOptM' b (prefixNatLikeFVars.map some)]
+      let hy' ← mkFreshExprMVar $ ← mkAppM ``LT.lt #[y', ← mkAppOptM' b (prefixNatLikeFVars.map some)]
+      let h ← mkFreshExprMVar $ ← mkAppM ``Eq #[← mkAppOptM' arg1 #[y], mkConst ``true]
+      let hf ← mkFreshExprMVar $ ← mkAppM ``Eq #[← mkAppOptM' fWithPrefix #[y'], mkConst ``true]
+      let innerLam ← mkLambdaFVars #[y', hy', hf] hf (binderInfoForMVars := .default)
+      let lamBody ← mkAppOptM ``ofMkFold1SomeLt #[none, inst, ← mkAppOptM' b (prefixNatLikeFVars.map some), fWithPrefix, fWithPrefix, innerLam, h, y, hy]
+      mkLambdaFVars #[y, hy, h] lamBody (binderInfoForMVars := .default)
+    | .leUpperBound b =>
+      let y ← mkFreshExprMVar t
+      let y' ← mkFreshExprMVar t
+      let hy ← mkFreshExprMVar $ ← mkAppM ``LE.le #[y, ← mkAppOptM' b (prefixNatLikeFVars.map some)]
+      let hy' ← mkFreshExprMVar $ ← mkAppM ``LE.le #[y', ← mkAppOptM' b (prefixNatLikeFVars.map some)]
+      let h ← mkFreshExprMVar $ ← mkAppM ``Eq #[← mkAppOptM' arg1 #[y], mkConst ``true]
+      let hf ← mkFreshExprMVar $ ← mkAppM ``Eq #[← mkAppOptM' fWithPrefix #[y'], mkConst ``true]
+      let innerLam ← mkLambdaFVars #[y', hy', hf] hf (binderInfoForMVars := .default)
+      let lamBody ← mkAppOptM ``ofMkFold1SomeLe #[none, inst, ← mkAppOptM' b (prefixNatLikeFVars.map some), fWithPrefix, fWithPrefix, innerLam, h, y, hy]
+      mkLambdaFVars #[y, hy, h] lamBody (binderInfoForMVars := .default)
+
+  trace[brute.debug] "bp5"
+
+  let (computationInnerLamOpt, computationRes, computationResIsTrue) ← buildComputationResBase binderInfosPrefix t f finalBinderInfo.b inst
+
+  trace[brute.debug] "bp5.5"
+
+  let arg3 ← buildArg3 prefixFVars prefixNatLikeFVars binderInfosPrefix finalBinderInfo f computationInnerLamOpt computationRes computationResIsTrue
+
+  trace[brute.debug] "bp6"
+
+  let res ←
+    match finalBinderInfo.b with
+    | .noUpperBound =>
+      let ofMkFold1Call ← mkAppOptM ``ofMkFold1None #[none, inst, fWithPrefix, arg1, arg2, arg3]
+      let lamBody ← mkAppOptM ``of_decide_eq_true #[none, none, ← mkAppOptM' ofMkFold1Call (finalBinderFVars.map some)]
+      mkLambdaFVars (prefixFVars ++ finalBinderFVars) lamBody (binderInfoForMVars := .default)
+    | .ltUpperBound b =>
+      let ofMkFold1Call ← mkAppOptM ``ofMkFold1SomeLt #[none, inst, ← mkAppOptM' b (prefixNatLikeFVars.map some), fWithPrefix, arg1, arg2, arg3]
+      let lamBody ← mkAppOptM ``of_decide_eq_true #[none, none, ← mkAppOptM' ofMkFold1Call (finalBinderFVars.map some)]
+      mkLambdaFVars (prefixFVars ++ finalBinderFVars) lamBody (binderInfoForMVars := .default)
+    | .leUpperBound b =>
+      let ofMkFold1Call ← mkAppOptM ``ofMkFold1SomeLe #[none, inst, ← mkAppOptM' b (prefixNatLikeFVars.map some), fWithPrefix, arg1, arg2, arg3]
+      let lamBody ← mkAppOptM ``of_decide_eq_true #[none, none, ← mkAppOptM' ofMkFold1Call (finalBinderFVars.map some)]
+      mkLambdaFVars (prefixFVars ++ finalBinderFVars) lamBody (binderInfoForMVars := .default)
+
+  return res
 
 @[tactic brute]
 def evalBrute : Tactic
 | `(tactic| brute) => withMainContext do
   let pf ← forallTelescope (← getMainTarget).consumeMData (cleanupAnnotations := true) $ fun xs g => do
     trace[brute.debug] "xs: {xs}, g: {g}"
-    let boundBinders ← popAllBoundBinders (xs.map Expr.fvarId!) #[]
-    /-  This version of `brute` produces a hardcoded proof which depends on the total number of bound binders.
-        If there are `N` bound binders, then `brute`:
-        - Builds a call to `mkFoldN`, with the appropriate arguments
-        - Compiles that call into a definition with the auxiliary definition `_brute`
-          - This step is required because `Lean.ofReduceBool`, the axiom which allows `brute` and `native_decide`
-            to trust the compiler's evaluation, requires that the argument it is provided is a constant. See
-            the docstrings for `Lean.ofReduceBool` and `Lean.reduceBool` for more details.
-        - Uses the compiler to confirm that the compiled definition evaluates to `true` (by invoking `Lean.ofReduceBool`)
-        - Constructs a proof term for the original goal using `ofMkFoldNEqTrue`
-
-       Each of the cases below are extremely similar, only substantively differing in which `mkFoldN` and
-       `ofMkFoldNEqTrue` constants to use. -/
-    match boundBinders with
-    | #[⟨x, b, hxb, inst⟩] =>
-      let boundFVars := #[.fvar x, .fvar hxb]
-      let natLikeFVars := #[.fvar x]
-      let unboundFVars := xs.filter (fun fvar => !boundFVars.contains fvar)
-      trace[brute.debug] "boundFVars: {boundFVars}, unboundFVars: {unboundFVars}"
-      let f ← mkLambdaFVars natLikeFVars (← mkDecide (← mkForallFVars unboundFVars g))
-      trace[brute.debug] "f: {f}"
-      let res ← mkAppOptM ``mkFold1 #[none, some inst, b, f, mkConst ``true]
-      trace[brute.debug] "res: {res}"
-
-      let levels := (collectLevelParams {} res).params.toList
-      let auxDeclName ← Term.mkAuxName `_brute
-      let decl := Declaration.defnDecl $
-        mkDefinitionValEx auxDeclName levels (mkConst ``Bool) res .abbrev .safe [auxDeclName]
-      addAndCompile decl
-
-      let rflPrf ← mkEqRefl (toExpr true)
-      let levelParams := levels.map .param
-      let foldResPf := mkApp3 (mkConst ``Lean.ofReduceBool) (mkConst auxDeclName levelParams) (toExpr true) rflPrf
-      let pf ← mkAppOptM ``ofMkFold1EqTrue #[none, some inst, b, f, foldResPf]
-      mkLambdaFVars boundFVars $ ← mkAppOptM ``of_decide_eq_true #[none, none, ← mkAppM' pf boundFVars]
-    | #[⟨x, b1, hxb1, inst1⟩, ⟨y, b2, hyb2, inst2⟩] =>
-      let boundFVars := #[.fvar x, .fvar hxb1, .fvar y, .fvar hyb2]
-      let natLikeFVars := #[.fvar x, .fvar y]
-      let unboundFVars := xs.filter (fun fvar => !boundFVars.contains fvar)
-      trace[brute.debug] "boundFVars: {boundFVars}, unboundFVars: {unboundFVars}"
-      let b2 ← mkLambdaFVars #[.fvar x] b2
-      let f ← mkLambdaFVars natLikeFVars (← mkDecide (← mkForallFVars unboundFVars g))
-      trace[brute.debug] "f: {f}"
-      let res ← mkAppOptM ``mkFold2 #[none, none, inst1, inst2, b1, b2, f, mkConst ``true]
-      trace[brute.debug] "res: {res}"
-
-      let levels := (collectLevelParams {} res).params.toList
-      let auxDeclName ← Term.mkAuxName `_brute
-      let decl := Declaration.defnDecl $
-        mkDefinitionValEx auxDeclName levels (mkConst ``Bool) res .abbrev .safe [auxDeclName]
-      addAndCompile decl
-
-      let rflPrf ← mkEqRefl (toExpr true)
-      let levelParams := levels.map .param
-      let foldResPf := mkApp3 (mkConst ``Lean.ofReduceBool) (mkConst auxDeclName levelParams) (toExpr true) rflPrf
-      let pf ← mkAppOptM ``ofMkFold2EqTrue #[none, none, inst1, inst2, b1, b2, f, foldResPf]
-      mkLambdaFVars boundFVars $ ← mkAppOptM ``of_decide_eq_true #[none, none, ← mkAppM' pf boundFVars]
-    | #[⟨x, b1, hxb1, inst1⟩, ⟨y, b2, hyb2, inst2⟩, ⟨z, b3, hzb3, inst3⟩] =>
-      let boundFVars := #[.fvar x, .fvar hxb1, .fvar y, .fvar hyb2, .fvar z, .fvar hzb3]
-      let natLikeFVars := #[.fvar x, .fvar y, .fvar z]
-      let unboundFVars := xs.filter (fun fvar => !boundFVars.contains fvar)
-      trace[brute.debug] "boundFVars: {boundFVars}, unboundFVars: {unboundFVars}"
-      let b2 ← mkLambdaFVars #[.fvar x] b2
-      let b3 ← mkLambdaFVars #[.fvar x, .fvar y] b3
-      let f ← mkLambdaFVars natLikeFVars (← mkDecide (← mkForallFVars unboundFVars g))
-      trace[brute.debug] "f: {f}"
-      let res ← mkAppOptM ``mkFold3 #[none, none, none, inst1, inst2, inst3, b1, b2, b3, f, mkConst ``true]
-      trace[brute.debug] "res: {res}"
-
-      let levels := (collectLevelParams {} res).params.toList
-      let auxDeclName ← Term.mkAuxName `_brute
-      let decl := Declaration.defnDecl $
-        mkDefinitionValEx auxDeclName levels (mkConst ``Bool) res .abbrev .safe [auxDeclName]
-      addAndCompile decl
-
-      let rflPrf ← mkEqRefl (toExpr true)
-      let levelParams := levels.map .param
-      let foldResPf := mkApp3 (mkConst ``Lean.ofReduceBool) (mkConst auxDeclName levelParams) (toExpr true) rflPrf
-      let pf ← mkAppOptM ``ofMkFold3EqTrue #[none, none, none, inst1, inst2, inst3, b1, b2, b3, f, foldResPf]
-      mkLambdaFVars boundFVars $ ← mkAppOptM ``of_decide_eq_true #[none, none, ← mkAppM' pf boundFVars]
-    | #[⟨x, b1, hxb1, inst1⟩, ⟨y, b2, hyb2, inst2⟩, ⟨z, b3, hzb3, inst3⟩, ⟨a, b4, hab4, inst4⟩] =>
-      let boundFVars := #[.fvar x, .fvar hxb1, .fvar y, .fvar hyb2, .fvar z, .fvar hzb3, .fvar a, .fvar hab4]
-      let natLikeFVars := #[.fvar x, .fvar y, .fvar z, .fvar a]
-      let unboundFVars := xs.filter (fun fvar => !boundFVars.contains fvar)
-      trace[brute.debug] "boundFVars: {boundFVars}, unboundFVars: {unboundFVars}"
-      let b2 ← mkLambdaFVars #[.fvar x] b2
-      let b3 ← mkLambdaFVars #[.fvar x, .fvar y] b3
-      let b4 ← mkLambdaFVars #[.fvar x, .fvar y, .fvar z] b4
-      let f ← mkLambdaFVars natLikeFVars (← mkDecide (← mkForallFVars unboundFVars g))
-      trace[brute.debug] "f: {f}"
-      let res ← mkAppOptM ``mkFold4
-        #[none, none, none, none, inst1, inst2, inst3, inst4, b1, b2, b3, b4, f, mkConst ``true]
-      trace[brute.debug] "res: {res}"
-
-      let levels := (collectLevelParams {} res).params.toList
-      let auxDeclName ← Term.mkAuxName `_brute
-      let decl := Declaration.defnDecl $
-        mkDefinitionValEx auxDeclName levels (mkConst ``Bool) res .abbrev .safe [auxDeclName]
-      addAndCompile decl
-
-      let rflPrf ← mkEqRefl (toExpr true)
-      let levelParams := levels.map .param
-      let foldResPf := mkApp3 (mkConst ``Lean.ofReduceBool) (mkConst auxDeclName levelParams) (toExpr true) rflPrf
-      let pf ← mkAppOptM ``ofMkFold4EqTrue
-        #[none, none, none, none, inst1, inst2, inst3, inst4, b1, b2, b3, b4, f, foldResPf]
-      mkLambdaFVars boundFVars $ ← mkAppOptM ``of_decide_eq_true #[none, none, ← mkAppM' pf boundFVars]
-    | #[⟨x, b1, hxb1, inst1⟩, ⟨y, b2, hyb2, inst2⟩, ⟨z, b3, hzb3, inst3⟩, ⟨a, b4, hab4, inst4⟩,
-        ⟨b, b5, hbb5, inst5⟩] =>
-      let boundFVars :=
-        #[.fvar x, .fvar hxb1, .fvar y, .fvar hyb2, .fvar z, .fvar hzb3, .fvar a, .fvar hab4, .fvar b, .fvar hbb5]
-      let natLikeFVars := #[.fvar x, .fvar y, .fvar z, .fvar a, .fvar b]
-      let unboundFVars := xs.filter (fun fvar => !boundFVars.contains fvar)
-      trace[brute.debug] "boundFVars: {boundFVars}, unboundFVars: {unboundFVars}"
-      let b2 ← mkLambdaFVars #[.fvar x] b2
-      let b3 ← mkLambdaFVars #[.fvar x, .fvar y] b3
-      let b4 ← mkLambdaFVars #[.fvar x, .fvar y, .fvar z] b4
-      let b5 ← mkLambdaFVars #[.fvar x, .fvar y, .fvar z, .fvar a] b5
-      let f ← mkLambdaFVars natLikeFVars (← mkDecide (← mkForallFVars unboundFVars g))
-      trace[brute.debug] "f: {f}"
-      let res ← mkAppOptM ``mkFold5
-        #[none, none, none, none, none, inst1, inst2, inst3, inst4, inst5, b1, b2, b3, b4, b5, f, mkConst ``true]
-      trace[brute.debug] "res: {res}"
-
-      let levels := (collectLevelParams {} res).params.toList
-      let auxDeclName ← Term.mkAuxName `_brute
-      let decl := Declaration.defnDecl $
-        mkDefinitionValEx auxDeclName levels (mkConst ``Bool) res .abbrev .safe [auxDeclName]
-      addAndCompile decl
-
-      let rflPrf ← mkEqRefl (toExpr true)
-      let levelParams := levels.map .param
-      let foldResPf := mkApp3 (mkConst ``Lean.ofReduceBool) (mkConst auxDeclName levelParams) (toExpr true) rflPrf
-      let pf ← mkAppOptM ``ofMkFold5EqTrue
-        #[none, none, none, none, none, inst1, inst2, inst3, inst4, inst5, b1, b2, b3, b4, b5, f, foldResPf]
-      mkLambdaFVars boundFVars $ ← mkAppOptM ``of_decide_eq_true #[none, none, ← mkAppM' pf boundFVars]
-    | _ => throwError "Not yet implemented (boundBinders: {boundBinders})"
+    let binderInfos ← popAllBoundBinders #[] (xs.map Expr.fvarId!) #[]
+    match binderInfos.toList with
+    | [] => throwError "Goal does not match the form required by brute, consider trying native_decide instead"
+    | [⟨x, b, hxbOpt, inst⟩] => bruteBaseCase1 xs g x b hxbOpt inst
+    | _ =>
+      let unboundFVars := xs.filter
+        (fun fvar =>
+          !(binderInfos.map (fun b => Expr.fvar b.x)).contains fvar &&
+          !((binderInfos.filterMap (fun b => b.hxb)).map Expr.fvar).contains fvar
+        )
+      bruteCore binderInfos unboundFVars g
   trace[brute.debug] "pf: {pf}"
   trace[brute.debug] "pf type: {← inferType pf}"
   let g ← getMainGoal
